src/tls/Crypto.AEAD.fsti
@@ -1,0 +1,37 @@
+module Crypto.AEAD
+
+module U8 = FStar.UInt8
+module Seq = FStar.Seq
+module EC = EverCrypt.AEAD
+module SC = Spec.AEAD
+module B = LowStar.Buffer
+module E = EverCrypt
+module U32 = FStar.UInt32
+module HS = FStar.HyperStack
+module HST = FStar.HyperStack.ST
+module EE = EverCrypt.Error
+module G = FStar.Ghost
+module MDM = FStar.Monotonic.DependentMap
+module F = Flags
+
+type plain_pred = (plain: Seq.seq SC.uint8) -> Tot Type0
+
+inline_for_extraction
+val state (a: SC.supported_alg) (phi: plain_pred) : Tot Type0
+
+val invariant (#a: SC.supported_alg) (#phi: plain_pred) (h: HS.mem) (s: state a phi) : GTot Type0
+
+val footprint (#a: SC.supported_alg) (#phi: plain_pred) (h: HS.mem) (s: state a phi) : GTot B.loc
+
+noextract
+inline_for_extraction
+let tag_len : (x: SC.alg) -> Tot (y: U32.t { U32.v y == SC.tag_length x }) =
+  let open SC in
+  function
+  | AES128_CCM8       ->  8ul
+  | AES256_CCM8       ->  8ul
+  | AES128_GCM        -> 16ul
+  | AES256_GCM        -> 16ul
+  | CHACHA20_POLY1305 -> 16ul
+  | AES128_CCM        -> 16ul
+  | AES256_CCM        -> 16ul
